ReductionOrderTheorems.v
@@ -1,6 +1,7 @@
 Require Export ReductionOrder.
 From stdpp Require Export relations.
 
+Require Import ReorderingTheorems.
 Require Import MyUtils.
 
 Section ReductionOrderTheorems.
@@ -193,20 +194,277 @@ Hint Resolve right_assoc_sym : gtr.
 Hint Resolve right_assoc_trans : gtr.
 
 Lemma gtrc_trans g oc1 oc2 oc3 t t' t'' :
-  gtrc g oc1 t t' → gtlc g oc2 t' t'' →
+  gtrc g oc1 t t' → gtrc g oc2 t' t'' →
   g.(rel) oc1 oc2 = Some Right_assoc → g.(rel) oc2 oc3 = Some Right_assoc →
   gtrc g oc3 t t''.
 Proof.
   intro. revert t'' oc2 oc3. induction H; intros.
   - inv H0.
-  - assert (rel g o oc3 = Some Right_assoc). { eauto using gtr. }
-    }
-    apply g.(left_assoc_sym) in H4 as ?.
-    inv H1; eauto with gtl.
-  - assert (rel g o oc3 = Some Left_assoc). {
-      eapply g.(left_assoc_trans). apply g.(left_assoc_sym). eassumption.
-      eapply g.(left_assoc_trans); eassumption.
-    }
-    apply g.(left_assoc_sym) in H5 as ?.
-    inv H2; eauto with gtl.
+  - assert (rel g o oc3 = Some Right_assoc). { eauto with gtr. }
+    apply g.(right_assoc_sym) in H4 as ?.
+    inv H1; eauto with gtr.
+  - assert (rel g o oc3 = Some Right_assoc). { eauto with gtr. }
+    apply g.(right_assoc_sym) in H5 as ?.
+    inv H2; eauto with gtr.
 Qed.
+
+Hint Resolve gtrc_trans : gtr.
+
+Lemma orc2_gtr_gtrc g t t1 t2 u u1 u2 (v : @parse_tree L O) o p oc :
+  u = INode u1 p u2 → t = INode t1 o t2 →
+  g.(rel) oc o = Some Right_assoc → g.(rel) o p ≠ Some Right_assoc →
+  gtr g u v → gtrc g oc t v.
+Proof.
+  intros. inv H3.
+  - inv H6. rename o' into q. rename t'1 into v1. rename t'2 into v2.
+    apply ORC2. assumption.
+    intro. destruct H2.
+    eauto with gtr.
+  - inv H5. apply ORC2. assumption.
+    intro. destruct H2.
+    eauto with gtr.
+  - inv H5. apply ORC2. assumption.
+    intro. destruct H2.
+    eauto with gtr.
+  - inv H6. apply ORC2. assumption.
+    intro. destruct H2.
+    eauto with gtr.
+Qed.
+
+Lemma gtrc_gtr_gtrc g o t u v :
+  gtrc g o t u → gtr g u v → gtrc g o t v.
+Proof.
+  intro. revert v. induction H; intros.
+  - inv H0.
+  - eauto using orc2_gtr_gtrc with gtr.
+  - inv H2; eauto with gtr.
+Qed.
+
+Lemma gtr_gtrc_gtrc g oc t u v :
+  gtr g t u → gtrc g oc u v → gtrc g oc t v.
+Proof.
+  intro. revert v. induction H; intros.
+  - inv H0. contradiction.
+    inv H1.
+    + eauto with gtr.
+    + apply ORC2. eauto with gtr.
+      intro. destruct H7. eauto with gtr.
+    + apply ORC3; eauto with gtr.
+      eauto 10 with gtr.
+  - inv H0; eauto with gtr.
+  - inv H0; eauto with gtr.
+  - inv H1; eauto with gtr.
+Qed.
+
+Lemma glr_trans g t t' t'' :
+  gtr g t t' → gtr g t' t'' → gtr g t t''.
+Proof.
+  intro. revert t''. induction H; intros.
+  - inv H1.
+    + eauto with gtr.
+    + inv H0; eauto using gtrc_gtr_gtrc with gtr.
+    + inv H0; eauto with gtr.
+    + inv H0; eauto using gtrc_gtr_gtrc with gtr.
+  - inv H0; eauto with gtr.
+    inv H6; eauto using gtr_gtrc_gtrc with gtr.
+  - inv H0; eauto with gtr.
+    inv H6; eauto with gtr.
+  - inv H1; eauto with gtr.
+    inv H7; eauto using gtr_gtrc_gtrc with gtr.
+Qed.
+
+Lemma gtrc_irreflexive g oc t t' :
+  gtrc g oc t t' → t ≠ t'.
+Proof.
+  intro. induction H; intro.
+  - inv H0.
+  - inv H1. contradiction.
+  - inv H2. contradiction.
+Qed.
+
+Inductive gtp_or_gtl g : parse_tree → parse_tree → Prop :=
+  | ULeft t u :
+      gtp g t u → gtp_or_gtl g t u
+  | URight t u :
+      gtl g t u → gtp_or_gtl g t u.
+
+Lemma asdfgh g t1 o t2 u1 p u2 u1' t1' :
+  g.(rel) o p = Some Left_assoc → gtlc g o t2 u2 →
+  yield (INode t1 o t2) = yield (INode u1 p u2) → yield u1 = yield u1' →
+  gtp g u1 u1' →
+  ∃ t1', gtp g t1 t1' ∧ yield t1 = yield t1'.
+Proof.
+  intros. apply yield_equivalence_are_reorderings in H1.
+  apply yield_equivalence_are_reorderings in H2.
+  induction H2; intros.
+
+  apply gtp_irreflexive in H3. contradiction.
+
+  
+  
+  subst. inv Hequ.
+  apply gtlc_irreflexive in H0. contradiction.
+
+  
+  
+
+Lemma gtp_commutes_gtl g t u v :
+  gtl g t u → gtp g u v → ∃ w, gtp g t w ∧ (rtc (gtp_or_gtl g)) w v.
+Proof.
+  intro. revert v. induction H; intros.
+  - inv H0. contradiction. clear H9.
+    rename t'1 into u1. rename o' into p. rename t'2 into u2.
+    inv H1.
+    + rename t'1 into v1, o' into q, t'2 into v2.
+      exists (INode v1 q v2). split.
+      apply OP1.
+      eapply priority_group_left_2. eassumption. eauto using left_assoc_sym.
+      apply rtc_refl.
+    + rename t1' into u1'.
+    
+    
+    
+    
+  (* AAAAAAAAAAAAAAAAAAAAA *)
+
+Lemma gtlc_gtr_gtlc g oc t u v :
+  (* g.(rel) oc oc' = Some Left_assoc → *)
+  gtlc g oc t u → gtr g u v → gtlc g oc t v.
+Proof.
+  intro. revert v. induction H; intros.
+  - inv H0.
+  - rename t'1 into u1, o' into p, t'2 into u2.
+    inv H1; eauto with gtl.
+    rename t'1 into v1, o' into q, t'2 into v2.
+    inv H7. contradiction.
+    apply OLC2. assumption.
+    apply g.(right_assoc_sym) in H6.
+    apply g.(right_assoc_group) with (o3 := oc) in H6.
+    intro. apply H6.
+    apply g.(left_assoc_sym). assumption.
+  - rename t'1 into u1, o' into p, t'2 into u2.
+    inv H2; eauto with gtl.
+    rename t'1 into v1, o' into q, t'2 into v2.
+    apply g.(right_assoc_sym) in H7.
+    apply g.(right_assoc_group) with (o3 := oc) in H7.
+    eauto with gtl.
+Qed.
+
+Lemma gtl_gtrc_gtrc g oc t u v :
+  gtl g t u → gtrc g oc u v → gtrc g oc t v.
+Proof.
+  intro. revert v. induction H; intros.
+  - rename t'1 into u1, o' into p, t'2 into u2.
+    assert (g.(rel) oc p = Some Right_assoc). {inv H1; assumption. }
+    apply g.(right_assoc_sym) in H2.
+    apply g.(right_assoc_group) with (o3 := o) in H2.
+    destruct H2.
+    eauto with gtl.
+  - inv H0; eauto with gtr.
+  - inv H0; eauto with gtr.
+  - inv H1; eauto with gtr.
+Qed.
+
+Create HintDb rel.
+Hint Resolve left_assoc_sym : rel.
+Hint Resolve right_assoc_sym : rel.
+Hint Resolve left_assoc_trans : rel.
+Hint Resolve right_assoc_trans : rel.
+Hint Resolve priority_trans : rel.
+Hint Resolve priority_group_left_1 : rel.
+(* Hint Resolve priority_group_left_2 : rel. *)
+Hint Resolve priority_group_right_1 : rel.
+(* Hint Resolve priority_group_right_2 : rel. *)
+
+(* Lemma gtlc_gtpr_gtlc g oc t u v :
+  gtlc g oc t u → gtpr g u v → gtlc g oc t v.
+Proof.
+  intro. revert v. induction H; intros.
+  - inv H0.
+  - rename t'1 into u1, o' into p, t'2 into u2.
+    inv H1.
+    + rename u0 into v1, p0 into q, u3 into v2.
+      destruct (g.(rel) o q) eqn:E. destruct d.
+      * apply OLC3; eauto with rel. *)
+        
+
+Lemma gtlc_gtpr_gtpr g oc t u v :
+  gtlc g oc t u → gtpr g u v → gtpr g t v.
+Proof.
+  intro. revert v. induction H; intros.
+  - inv H0.
+  - rename t'1 into u1, o' into p, t'2 into u2.
+    inv H1.
+    + rename u0 into v1, p0 into q, u3 into v2.
+      
+
+Lemma gtpr_trans g t u v :
+  gtpr g t u → gtpr g u v → gtpr g t v.
+Proof.
+  intro. revert v. induction H; intros.
+  - inv H0; eauto using GTPR_Priority with rel.
+  - inv H0. contradiction.
+    inv H1.
+    + rename u0 into v1, p0 into q, u3 into v2.
+      apply GTPR_Priority.
+      eauto using g.(priority_group_left_2) with rel.
+    + rename u0 into v1, p0 into q, u3 into v2.
+      inv H7. contradiction.
+      apply GTPR_LAssoc.
+      eauto with rel.
+      apply OLC3; eauto using gtlc_trans with rel.
+    + rename u0 into v1, p0 into q, u3 into v2.
+      exfalso.
+      apply g.(right_assoc_group) with (o3 := o) in H5.
+      apply H5. auto with rel.
+    + rename t1' into u1'.
+      apply GTPR_LAssoc. assumption.
+      apply OLC3; assumption.
+    + (* POSSIBLE CHEAT HERE *)
+      rename t2' into u2'.
+      eapply GTPR_Temp. assumption.
+      apply OLC3; eassumption.
+      assumption.
+    + (* POSSIBLE CHEAT HERE *)
+      rename t1' into u1', t2' into u2'.
+      eapply GTPR_Temp. assumption.
+      apply OLC3; try eassumption.
+      assumption.
+    + (* CHEAT CASE *)
+      rename u0 into v1, p0 into q, u3 into v2.
+      rename u2' into v2'.
+      eapply GTPR_Temp. eauto with rel.
+      apply OLC3; eauto with rel.
+      inv H7. contradiction.
+
+
+Lemma gtl_gtr_cotrans g t u v :
+  gtl g t u → gtr g u v → gtl g t v ∨ gtr g t v.
+Proof.
+  intro. revert v. induction H; intros.
+  - rename t'1 into u1. rename o' into p. rename t'2 into u2.
+    inv H1.
+    + apply g.(left_assoc_sym) in H.
+      apply g.(left_assoc_group) with (o3 := o') in H.
+      contradiction.
+    + left. apply OL1. assumption.
+      apply OLC3; eauto with gtl.
+      inv H0. contradiction. assumption.
+    + rename t2' into u2'. inv H0. contradiction.
+      left. apply OL1. assumption.
+      apply OLC3; eauto with gtl.
+      eauto using gtlc_gtr_gtlc.
+    + rename t1' into u1', t2' into u2'. inv H0. contradiction.
+      left. apply OL1. assumption.
+      apply OLC3; eauto with gtl.
+      eauto using gtlc_gtr_gtlc.
+  - inv H0.
+    + rename t'1 into v1, o' into q, t'2 into v2.
+      inv H6. contradiction.
+      right. apply OR1. assumption.
+      apply ORC3; auto.
+      eauto using gtl_gtrc_gtrc.
+    + rename t1'0 into t1''.
+      apply IHgtl in H5. destruct H5; auto with gtl gtr.
+    + left. (* FUCKING KUUUUT*)
+
